Foundation/Propositional/Heyting/Semantics.lean
@@ -1,4 +1,4 @@
-import Foundation.Propositional.Hilbert.WellKnown
+import Foundation.Propositional.Hilbert.Basic
 import Foundation.Vorspiel.Order
 import Foundation.Logic.LindenbaumAlgebra
 
@@ -93,68 +93,62 @@ lemma val_not (φ : Formula α) : ℍ ⊧ ∼φ ↔ (ℍ ⊧ₕ φ) = ⊥ := by
 @[simp] lemma val_or (φ ψ : Formula α) : ℍ ⊧ φ ⋎ ψ ↔ (ℍ ⊧ₕ φ) ⊔ (ℍ ⊧ₕ ψ) = ⊤ := by
   simp [val_def]; rfl
 
-def mod (H : Hilbert α) : Set (HeytingSemantics α) := Semantics.models (HeytingSemantics α) H.axiomInstances
+def mod (Ax : Axiom α) : Set (HeytingSemantics α) := Semantics.models (HeytingSemantics α) Ax.instances
 
-variable {H : Hilbert α}
+variable {Ax : Axiom α}
 
 lemma mod_models_iff {φ : Formula α} :
-    mod.{_,w} H ⊧ φ ↔ ∀ ℍ : HeytingSemantics.{_,w} α, ℍ ⊧* H.axiomInstances → ℍ ⊧ φ := by
+    mod.{_,w} Ax ⊧ φ ↔ ∀ ℍ : HeytingSemantics.{_,w} α, ℍ ⊧* Ax.instances → ℍ ⊧ φ := by
   simp [mod, Semantics.models, Semantics.set_models_iff]
 
-lemma sound {φ : Formula α} (d : H ⊢! φ) : mod H ⊧ φ := by
+lemma sound {φ : Formula α} (d : (Hilbert Ax) ⊢! φ) : mod (Hilbert Ax) ⊧ φ := by
   apply mod_models_iff.mpr;
   intro ℍ hℍ;
   induction d with
   | @axm φ s hφ =>
     apply hℍ.RealizeSet;
     use φ;
-    simpa;
+    grind;
   | @mdp φ ψ _ _ ihpq ihp =>
     have : (ℍ ⊧ₕ φ) ≤ (ℍ ⊧ₕ ψ) := by simpa using ihpq
     simpa [val_def'.mp ihp] using this
   | _ => simp [himp_himp_inf_himp_inf_le, himp_inf_himp_inf_sup_le]
 
-instance : Sound H (mod H) := ⟨sound⟩
+instance : Sound (Hilbert Ax) (mod (Hilbert Ax)) := ⟨sound⟩
 
 section
 
 open Entailment.LindenbaumAlgebra
 
-variable [DecidableEq α] (H : Hilbert α) [H.HasEFQ] [Entailment.Consistent H]
+variable [DecidableEq α] {Ax : Axiom α} [Ax.HasEFQ] [Entailment.Consistent (Hilbert Ax)]
 
-def lindenbaum : HeytingSemantics α where
-  Algebra := Entailment.LindenbaumAlgebra H
+def lindenbaum (Ax : Axiom α) [Ax.HasEFQ] [Entailment.Consistent (Hilbert Ax)] : HeytingSemantics α where
+  Algebra := Entailment.LindenbaumAlgebra (Hilbert Ax)
   valAtom a := ⟦.atom a⟧
 
-
-lemma lindenbaum_val_eq : (lindenbaum H ⊧ₕ φ) = ⟦φ⟧ := by
+lemma lindenbaum_val_eq : (lindenbaum Ax ⊧ₕ φ) = ⟦φ⟧ := by
   induction φ with
   | hand φ ψ ihp ihq => simp only [hVal_and, ihp, ihq]; rw [inf_def];
   | hor _ _ ihp ihq => simp only [hVal_or, ihp, ihq]; rw [sup_def];
   | himp _ _ ihp ihq => simp only [hVal_imply, ihp, ihq]; rw [himp_def];
   | _ => rfl
 
-variable {H}
-
-omit [Entailment.Consistent H] in
-lemma lindenbaum_complete_iff [Entailment.Consistent H] {φ : Formula α} : lindenbaum H ⊧ φ ↔ H ⊢! φ := by
+lemma lindenbaum_complete_iff {φ : Formula α} : lindenbaum Ax ⊧ φ ↔ (Hilbert Ax) ⊢! φ := by
   simp [val_def', lindenbaum_val_eq, provable_iff_eq_top]
 
-instance : Sound H (lindenbaum H) := ⟨lindenbaum_complete_iff.mpr⟩
+instance : Sound (Hilbert Ax) (lindenbaum Ax) := ⟨lindenbaum_complete_iff.mpr⟩
 
-instance : Complete H (lindenbaum H) := ⟨lindenbaum_complete_iff.mp⟩
+instance : Complete (Hilbert Ax) (lindenbaum Ax) := ⟨lindenbaum_complete_iff.mp⟩
 
 end
 
-open Hilbert.Deduction
-
-lemma complete [DecidableEq α] {φ : Formula α} [H.HasEFQ] (h : mod.{_,u} H ⊧ φ) : H ⊢! φ := by
-  wlog Con : Entailment.Consistent H
+lemma complete [DecidableEq α] [Ax.HasEFQ] {φ : Formula α} (h : mod.{_,u} Ax ⊧ φ) : (Hilbert Ax) ⊢! φ := by
+  wlog Con : Entailment.Consistent (Hilbert Ax)
   . exact Entailment.not_consistent_iff_inconsistent.mp Con φ
   exact lindenbaum_complete_iff.mp <|
-    mod_models_iff.mp h (lindenbaum H) ⟨fun ψ hψ ↦ lindenbaum_complete_iff.mpr <| Hilbert.axm_instances! hψ⟩
+    mod_models_iff.mp h (lindenbaum Ax) ⟨fun ψ hψ ↦ lindenbaum_complete_iff.mpr <| by grind⟩
 
-instance [DecidableEq α] [H.HasEFQ] : Complete H (mod.{_,u} H) := ⟨complete⟩
+instance [DecidableEq α] [Ax.HasEFQ] : Complete (Hilbert Ax) (mod.{_,u} Ax) := ⟨complete⟩
 
 end HeytingSemantics
 
