Foundation/Modal/ModalCompanion/Int.lean
@@ -17,14 +17,14 @@ lemma Kripke.sound_frameClass_of_equiv (L₁ L₂ : Logic ℕ) [L₁ ≊ L₂] {
 lemma Kripke.complete_frameClass_of_equiv (L₁ L₂ : Logic ℕ) [L₁ ≊ L₂] {C : Kripke.FrameClass} [Complete L₁ C] : Complete L₂ C := by grind;
 
 
-lemma gS4_of_Int : Hilbert.Int ⊢! φ → Modal.S4 ⊢! φᵍ := by
-  apply provable_goedelTranslated_of_provable Hilbert.Int Modal.S4;
+lemma gS4_of_Int : Propositional.Int ⊢! φ → Modal.S4 ⊢! φᵍ := by
+  apply provable_goedelTranslated_of_provable;
   rintro _ ⟨φ, ⟨_⟩, ⟨s, rfl⟩⟩;
   apply nec! $ efq!;
 
 namespace S4
 
-instance : Modal.S4 ≊ 𝐈𝐧𝐭.smallestMC := by
+instance : Modal.S4 ≊ Propositional.Int.smallestMC := by
   apply Logic.equiv_of_provable;
   intro φ;
   constructor;
@@ -45,11 +45,11 @@ instance : Modal.S4 ≊ 𝐈𝐧𝐭.smallestMC := by
       apply gS4_of_Int;
       simpa [theory, Propositional.Logic.iff_provable, Set.mem_setOf_eq] using hφ;
 
-lemma eq_smallestMC_of_Int : Modal.S4 = 𝐈𝐧𝐭.smallestMC := Logic.eq_of_equiv
+lemma eq_smallestMC_of_Int : Modal.S4 = Propositional.Int.smallestMC := Logic.eq_of_equiv
 
-instance : Sound 𝐈𝐧𝐭.smallestMC FrameClass.S4 := Kripke.sound_frameClass_of_equiv Modal.S4 𝐈𝐧𝐭.smallestMC
+instance : Sound Propositional.Int.smallestMC FrameClass.S4 := Kripke.sound_frameClass_of_equiv Modal.S4 Propositional.Int.smallestMC
 
-instance : ModalCompanion 𝐈𝐧𝐭 Modal.S4 := by
+instance : ModalCompanion Propositional.Int Modal.S4 := by
   apply eq_smallestMC_of_Int ▸
     Modal.instModalCompanion_of_smallestMC_via_KripkeSemantics
     Propositional.Kripke.FrameClass.all
@@ -62,14 +62,14 @@ end S4
 
 
 
-instance : 𝐈𝐧𝐭.smallestMC ⪯ Modal.Grz := calc
+instance : Propositional.Int.smallestMC ⪯ Modal.Grz := calc
   _ ≊ Modal.S4  := by symm; infer_instance;
   _ ⪯ Modal.Grz := inferInstance
 
 
 namespace Grz
 
-instance : Modal.Grz ≊ 𝐈𝐧𝐭.largestMC := by
+instance : Modal.Grz ≊ Propositional.Int.largestMC := by
   apply Logic.equiv_of_provable;
   intro φ;
   constructor;
@@ -87,11 +87,11 @@ instance : Modal.Grz ≊ 𝐈𝐧𝐭.largestMC := by
     | mem₁ h => apply WeakerThan.pbl h;
     | mem₂ h => rcases h with ⟨φ, hφ, rfl⟩; simp;
 
-lemma is_largestMC_of_Int : Modal.Grz = 𝐈𝐧𝐭.largestMC := Logic.eq_of_equiv
+lemma is_largestMC_of_Int : Modal.Grz = Propositional.Int.largestMC := Logic.eq_of_equiv
 
-instance : Sound 𝐈𝐧𝐭.largestMC FrameClass.finite_Grz := Kripke.sound_frameClass_of_equiv Modal.Grz 𝐈𝐧𝐭.largestMC
+instance : Sound Propositional.Int.largestMC FrameClass.finite_Grz := Kripke.sound_frameClass_of_equiv Modal.Grz Propositional.Int.largestMC
 
-instance : ModalCompanion 𝐈𝐧𝐭 Modal.Grz := by
+instance : ModalCompanion Propositional.Int Modal.Grz := by
   apply is_largestMC_of_Int ▸ Modal.instModalCompanion_of_largestMC_via_KripkeSemantics
     Propositional.Kripke.FrameClass.finite_all
     FrameClass.finite_Grz
@@ -102,14 +102,14 @@ instance : ModalCompanion 𝐈𝐧𝐭 Modal.Grz := by
 end Grz
 
 
-lemma iff_provable_Cl_provable_dia_gS4 : 𝐂𝐥 ⊢! φ ↔ Modal.S4 ⊢! ◇φᵍ := by
+lemma iff_provable_Cl_provable_dia_gS4 : Propositional.Cl ⊢! φ ↔ Modal.S4 ⊢! ◇φᵍ := by
   constructor;
   . intro h;
     suffices Modal.S4 ⊢! □◇φᵍ by exact axiomT'! this;
-    have : Modal.S4 ⊢! (∼∼φ)ᵍ := ModalCompanion.companion.mp $ iff_negneg_Int_Cl.mpr h;
+    have : Modal.S4 ⊢! (∼∼φ)ᵍ := ModalCompanion.companion.mp $ glivenko.mpr h;
     cl_prover [this];
   . intro h;
-    apply iff_negneg_Int_Cl.mp;
+    apply glivenko.mp;
     suffices Modal.S4 ⊢! (∼∼φ)ᵍ by exact ModalCompanion.companion.mpr this;
     replace h : Modal.S4 ⊢! □◇φᵍ := nec! h;
     cl_prover [h];
@@ -117,7 +117,7 @@ lemma iff_provable_Cl_provable_dia_gS4 : 𝐂𝐥 ⊢! φ ↔ Modal.S4 ⊢! ◇�
 /--
   Chagrov & Zakharyaschev 1997, Theorem 3.89
 -/
-theorem embedding_Int_GL : 𝐈𝐧𝐭 ⊢! φ ↔ Modal.GL ⊢! φᵍᵇ:= Iff.trans ModalCompanion.companion iff_boxdot_GL_Grz.symm
+theorem embedding_Int_GL : Propositional.Int ⊢! φ ↔ Modal.GL ⊢! φᵍᵇ:= Iff.trans ModalCompanion.companion iff_boxdot_GL_Grz.symm
 
 
 end LO.Modal
